\section{Spectral decomposition}
The transfer function of a state-space system $\mathbf{G(s)}$, can be expressed as equation~\eqref{ss2tf},
\begin{equation}
 \bm{G(s)} = \bm{C} \: (s\bm{I} - \bm{A})^{-1} \: \bm{B} + \bm{D} \text{.}
  \label{ss2tf}
\end{equation}
where $\bm{A}, \bm{B}, \bm{C}, \bm{D}$  are state-space matrices in minimum realization. Let $\bm{A}$  have no repeated eigenvalues. Then, from \cite{Sko05}, $\bm{A}$ can be written as:
\begin{equation}
%\begin{align*}
\bm{A} = \sum_{i=1}^n \lambda_i \: \bm{t}_i\: \bm{q}_i^H 
%\end{align*}
\label{specDec1}
\end{equation}

According to the Shifting Theorem \cite{Bha12}, the eigenvalues of $s\bm{I}-\bm{A}$ are $s-\lambda$ and the eigenvectors of $s\bm{I}-\bm{A}$ and $\bm{A}$ remain the same. Thus, we can write,
\begin{align*}
  s\bm{I} - \bm{A} = \sum_{i=1}^n (s - \lambda_i) \: \bm{t}_i\: \bm{q}_i^H   
\end{align*}
    Assuming all eigenvalues are non-zero, the eigenvalues of $\bm{A}^{-1}$ are ${\frac{1}{\lambda_1},\frac{1}{\lambda_2}....,\frac{1}{\lambda_n}}$ and eigenvalues of $(s\bm{I} - \bm{A})^{-1}$ are ${\frac{1}{s-\lambda_1},\frac{1}{s-\lambda_2}....,\frac{1}{s-\lambda_n}}$. Additionally, the same matrix diagonalizes $(s\bm{I} - \bm{A})^{-1}$ and $\bm{A}$ (Appendix A.2.1 in \cite{Sko05}). Thus, $(s\bm{I} - \bm{A})^{-1}$ and $\bm{A}$ will have the same eigenvectors. We can now write,
\begin{equation}
(s\bm{I} - \bm{A})^{-1} = \sum_{i=1}^n \frac{\bm{t}_i\: \bm{q}_i^H}{s - \lambda_i} 
\label{specDec2}
\end{equation}
We know the input and output pole vectors as
\begin{align*}
\bm{y}_{pi} = \bm{C}\bm{t_i} \\
\bm{u}_{pi}= \bm{q}_{i}^H\bm{B} 
\end{align*}
Thus, equation~\eqref{ss2tf} can be reformulated as,
\begin{align*}
\bm{G(s)} &=  \bm{C} \: (s\bm{I} - \bm{A})^{-1} \: \bm{B} + \bm{D} \\
	&= \bm{C}\: \sum_{i=1}^n \frac{\bm{t}_i\: \bm{q}_i^H}{(s - \lambda_i)}\: \bm{B} + \bm{D} \\
	&= \sum_{i=1}^n \frac{\bm{C}\: \bm{t}_i\: \bm{q}_i^H\: \bm{B}}{s - \lambda_i} + \bm{D} \\
    &= \sum_{i=1}^n \frac{\bm{y}_{pi}\: \bm{u}_{pi}^H}{s - \lambda_i} + \bm{D} 
\end{align*}
\textbf{Hence, proven.}

\begin{flushleft}
Testing for a random plant $\bm{A}$ with 3 states: 
\begin{align*}
\bm{A} &=
\begin{bmatrix}
2 & 1 & -0.5 \\
1 & -1 & 0 \\
-0.5 & 0 & -4 
\end{bmatrix},
\end{align*}
in the case of SISO;
\begin{align*}
\bm{B} = 
\begin{bmatrix}
1 \\
0 \\
2 
\end{bmatrix},
\bm{C} = 
 \begin{bmatrix}
1 & -1 & 2 
\end{bmatrix},
\bm{D} = \bm{0}
\end{align*}
\begin{figure}
    \centering
    \begin{tikzpicture}
    \input{images/q211SISO}
    \end{tikzpicture}
    \caption{SISO Plant Response to a decaying input, $u = 2e^{-t}$.}
    \label{siso}
\end{figure}
and MIMO (TITO);
\begin{align*}
\bm{B} = 
\begin{bmatrix}
-1 & 0 \\
4 & -2 \\
0 & 1 
\end{bmatrix},
\bm{C} = 
 \begin{bmatrix}
2 & 0 & 0 \\
1 & -1 & 2 \\
\end{bmatrix},
\bm{D} = 
 \begin{bmatrix}
0 & 0 \\
0 & 0 \\
\end{bmatrix}
\end{align*}
\begin{figure}
    \centering
    \begin{tikzpicture}
    \input{images/q211MIMO}
    \end{tikzpicture}
    \caption{MIMO Plant Response to a decaying input, $u = [2e^{-t}\: 0]^T$. }
    \label{mimo}
\end{figure}

As both figures \ref{siso} and \ref{mimo} show, the spectral decomposition and the standard \emph{ss2tf()} function in matlab leads to the same plants with the same responses to inputs.
\end{flushleft}