%%%%%%%%%%%%%%%%%%%%%%%%%%%%%%%%%%%%%%%%%%%%%%%%%%%%%%%%%%%%%%%%%%%%%%%%%%%%%%%
%  Coursework template                                                        %
%  Advanced Control Systems lecture, RWTH Aachen University                   %
%  Version 1.01, 2014                                                         %
%%%%%%%%%%%%%%%%%%%%%%%%%%%%%%%%%%%%%%%%%%%%%%%%%%%%%%%%%%%%%%%%%%%%%%%%%%%%%%%

\documentclass{scrreprt}

\include{title}

\include{packages}

%%%%%%%%%%%%%%%%%%%%%%%%%%% DO NOT MODIFY THIS PART %%%%%%%%%%%%%%%%%%%%%%%%%%%

\subtitle{Coursework}
\makeatletter
\let\runauthor\@author
\let\runtitle\@title
\makeatother

\newcommand{\taskapp}{Task}
\renewcommand*\chapterformat{\taskapp~\thechapter:~}

\titleformat{\section}{\large\bfseries}{}{0pt}{Question \thesection:~}

\fancypagestyle{plain}{
  \fancyhf{}
  \fancyhead[C]{\runtitle}
	\fancyhead[R]{\thepage}
	\fancyhead[L]{\runauthor}
}

\begin{document}

%% Titlepage
\maketitle

%% Table of contents
\tableofcontents 

\cleardoublepage

\pagestyle{plain}

%%%%%%%%%%%%%%%%%%%%%%%%%%%%% Content starts here %%%%%%%%%%%%%%%%%%%%%%%%%%%%%

\chapter{System Analysis}
\input{Content/211}

\input{Content/212}

\input{Content/213}

\chapter{MIMO-systems}

\section{Proof of equivalence}
Let $\bm{F}(s) \equiv \mathcal{F}_l(\bm{P},\bm{K})$ \\
then, $||\bm{F}(s)||_2 = \sqrt{\frac{1}{2\:\pi}\: \int_{-\infty}^{\infty}\: trace[\bm{F}(\omega)\:\bm{F}(\omega)^H]}d\omega$
\\
\begin{figure}[htb]
  \centering
  \tikzstyle{block}     = [draw, rectangle, minimum height=1cm, minimum width=1.2cm]
    \tikzstyle{branch}    = [circle, inner sep=0pt, minimum size=1mm, fill=black, draw=black]
    \tikzstyle{connector} = [->, thin]
    \tikzstyle{dummy}     = [inner sep=0pt, minimum size=0pt]
    \tikzstyle{inout}     = []
    \tikzstyle{sum}       = [circle, inner sep=0pt, minimum size=2mm, draw=black, thick]
    \begin{tikzpicture}[auto, node distance=1cm, >=stealth']
      \node[block] (P) {$\bm{P}$};
      \node[block] (K) [below=of P] {$\bm{K}$};
      \node[inout] (w) [left=of P] {$\bm{w}$};
      \node[inout] (zeta) [right=of P] {$\bm{\zeta}$};
      \draw[->] (K.west) -| ++(-1,1) node {$\bm{\:\:\:\:\:u}$} |- (P.210);
      \draw[->] (P.-30) -| ++(1,-1) node {$\bm{\:\:\:\:\:v}$} |- (K.east);
 	 \draw[connector] (P.0) -- (zeta);
	 \draw[connector] (w) -- (P.180);
    \end{tikzpicture}
	  \caption{Simple MIMO block diagram for plant P and controller K}
    \label{fig:blockDiagram}
\end{figure} \\
From ~\ref{fig:blockDiagram} we can derive the following:
\begin{align*}
\bm{\zeta}(s) &= \mathcal{F}_l(\bm{P},\bm{K})\: \bm{w} \\
	&= \bm{F}(s)\:\bm{w}(s)
\end{align*}
Average power of any random process $x(t)$,
\begin{align*}
P_x = E\:\lim_{T\to\infty} \frac{1}{2T}\:\int_{-T}^T\: x(t)^2\:dt \\
\end{align*}
For a stochastic stationary process,
\begin{align*}
P_x &= \lim_{T\to\infty} \frac{1}{2T}\:\int_{-T}^T\: E\:x(t)^2\:dt \\
	&= R_x\:(\tau=0) \ \ where,\\
R_x &= E[x(t)\:\bar{x}(t)] \\
\end{align*}
if $\bm{x}(t)$ is a vector,
\begin{equation}
\bm{R_x}(\tau) = trace[\bm{x}(t + \tau)\: \bm{x}(t)^H]
\end{equation}
Average power of $\bm{\zeta}(t)$:
\begin{equation}
P_{\zeta} = E\:\lim_{T\to\infty} \frac{1}{2T}\:\int_{-T}^T\: \bm{z}(t)^T\: \bm{z}(t)dt \\
\end{equation}
Stochastic stationary process assumed, first part can be proven as follows;
\begin{align*}
\bm{R}_{z}(\tau=0) &= E\:\lim_{T\to\infty} \frac{1}{2T}\:\int_{-T}^T\: \bm{z}(t)^T\: \bm{z}(t)dt \\
\bm{R}_{z}(\tau) &= trace[E\:\bm{\zeta}(t + \tau)\: \bm{\zeta}(t)^H] \\
\bm{R}_{z}(\tau=0) &= trace[E\:\bm{z}(t)\: \bm{z}(t)^H]
\end{align*}
Spectral power density;
\begin{align*}
P_w &= trace[\bm{R}_w(\tau=0)] \\
	&= trace[E\:\bm{w}(t)\: \bm{w}(t)^T] \\
\bm{R}_w &= \frac{1}{2\pi}\: \int_{-\infty}^{\infty}\: \bm{S}_w(j\omega)\: e^{(j2\pi\tau\omega)}\:d\omega \\
P_w &= \frac{1}{2\pi}\: \int_{-\infty}^{\infty}\: trace(\bm{S}_w(j\omega))\: d\omega
\end{align*}
for a stable LTI system, if $\bm{S}_{\zeta}=\bm{F}\bm{S}_w\bm{F}^H$, then
\begin{align*}
P_z &= \frac{1}{2\pi}\: \int_{-\infty}^{\infty}\: trace[\bm{F}(j\omega)\bm{S}_w(j\omega)\bm{F}(j\omega)^H]\: d\omega
\end{align*}
Now, let $\bm{w}(t)$ be white noise of unit Intensity, $\bm{S}_w(j\omega)=\bm{I}$ and \\
$\bm{R}_w(\tau)= \bm{I}\delta(t - \tau)=E[\bm{w}(t)\bm{w}(t)^T]$, thus
\begin{align*}
P_z &= \frac{1}{2\pi}\: \int_{-\infty}^{\infty}\: trace[\bm{F}(j\omega)\bm{F}(j\omega)^H]\: d\omega \\
	&= ||\bm{F}(s)||_2^2 \\
	&= ||\mathcal{F}_l(\bm{P},\bm{K})||^2
\end{align*}

\section{System zero and down squaring}
From the given state-space system in minimum realisation and inserting the system matrices in ~\eqref{eq:T}, we can write the transfer function matrix as follows:
\begin{align*}
\bm{G}(s)&=
\begin{bmatrix}
\frac{s - 1}{s - 2} & \frac{s + 1}{s + 2} \\
\end{bmatrix}\\
M_1 &= \frac{s - 1}{s - 2} \: and \: M_2 = \frac{s + 1}{s + 2} \\
\end{align*}
Using Polynomial Matrix $\bm{P}(s)$: \\
\begin{align*}
\bm{P}(s) &=
\begin{bmatrix}
s\bm{I}-\bm{A} & -\bm{B} \\
\bm{C} & \bm{D} \\
\end{bmatrix}
=
\begin{bmatrix}
s - 2 & 0 & -1 & 0 \\
0 & s + 2 & 0 & -1 \\
1 & -1 & 1 & 1
\end{bmatrix} \\
\\
\bm{P}(s=1) &=
\begin{bmatrix}
 -1 & 0 & -1 & 0 \\
0 & 3 & 0 & -1 \\
1 & -1 & 1 & 1
\end{bmatrix},
\bm{P}(s=-1) =
\begin{bmatrix}
 -3 & 0 & -1 & 0 \\
0 & 1 & 0 & -1 \\
1 & -1 & 1 & 1
\end{bmatrix}
\end{align*}
Since  $\bm{P}(s)$ is always of full rank, there is no transmission zero. \\
\\
Using Pre-compensator and invoking p-z cancellations in LHP:\\
\begin{align*}
k_1 = \alpha, \: k_2 = \beta\:\frac{s+2}{s-2}
\end{align*}
\begin{align*}
\bm{G}_{s}(s) &= k_1(\frac{s-1}{s-2}) + k_2(\frac{s+1}{s+2}) \\
	&= \frac{\alpha\:s - \alpha + \beta\:s + \beta}{s-2} \\
	&= \frac{(\alpha + \beta)\:s + (\beta-\alpha)}{s-2} \\
hence,\\
s &= \frac{-(\beta-\alpha)}{\alpha+\beta}
\end{align*}
for $\beta>\alpha>0$, system zero is in open LHP and no RHP p-z cancellations.
\section{Euclids algorithm}
The given transfer function can be factorised as follows:
\begin{equation}
G(s) = \frac{s-1}{(s+2)(s-2)(s+1)}
 \label{eq:G}
\end{equation}
From ~\eqref{eq:G} we can see that there exists a pole in the RHP, hence it is an unstable plant.
let $s=\frac{1-\lambda}{\lambda}$,
\begin{align*}
s+2 &= \frac{1-\lambda+2\:\lambda}{\lambda}, \: s-2 = \frac{1-\lambda-2\:\lambda}{\lambda}, \: s+1 = \frac{1-\lambda+\lambda}{\lambda}, \: s-1 = \frac{1-\lambda-\lambda}{\lambda} \\
s+2 &= \frac{1+\lambda}{\lambda}, \: s-2 = \frac{1-3\:\lambda}{\lambda}, \: s+1 = \frac{1}{\lambda}, \: s-1 = \frac{1-2\:\lambda}{\lambda}\\
\tilde{G}(\lambda) &= \frac{\lambda^2(1-2\:\lambda)}{(1-\lambda)(1-3\:\lambda)}
\end{align*}
The coprime polynomials $n(\lambda)$ and $m(\lambda)$ can be expressed as:
\begin{align*}
n(\lambda) = \lambda^2 - 2\:\lambda^3 \:,\: m(\lambda) = 1-2\:\lambda-3\:\lambda^2\\
\end{align*}
degree(n)$>$degree(m), let $n=mq_1 + r_1$ and $m=r_1q_2 + r_2$, we get:
\begin{align*}
\lambda^2 - 2\:\lambda^3 = (1-2\:\lambda-3\:\lambda^2)q_1 + r_1\\
q_1 = \frac{2\lambda}{3} - \frac{7}{9}\: ,\: r_1 = \frac{7}{9} - \frac{20\lambda}{9}\\
\\
1-2\:\lambda-3\:\lambda^2 =  (\frac{7-20\lambda}{9})q_2 + r_2\\
q_2 = \frac{27\lambda}{20} + \frac{549}{400}\: ,\: r_2 = \frac{-27}{400}\\
\end{align*}
solving for $r_2$:
\begin{align*}
r_2 &= -q_2n + (1+q_1q_2)m \\
1 &= (\frac{-q_2}{r_2})n + (\frac{1+q_1q_2}{r_2})m\\
u(\lambda) &= \frac{-q_2}{r_2} = \frac{\frac{-27\:\lambda}{20} - \frac{549}{400}}{\frac{-27}{400}}\\
	&= 20\lambda + \frac{61}{3} \\
\\
v(\lambda) &= \frac{1+q_1q_2}{r_2} = \frac{1+ (\frac{2\lambda}{3} - \frac{7}{9})( \frac{27\lambda}{20} + \frac{549}{400})}{\frac{-27}{400}}\\
	&= \frac{-40}{3}\lambda^2+2\lambda+1\\
\end{align*}
Using $\lambda = \frac{1}{s+1}$;\\
\begin{equation}
N(s) = \frac{s-1}{(s+1)^3}\\
 \label{eq:n}
\end{equation}
\begin{equation}
M(s) = \frac{(s+2)(s-2)}{(s+1)^2}\\
 \label{eq:m}
\end{equation}
\begin{equation}
U(s) = \frac{61s+121}{3(s+1)}\\
 \label{eq:u}
\end{equation}
\begin{equation}
V(s) = \frac{3s^2+12s-31}{3(s+1)^2}
 \label{eq:v}
\end{equation}
From equations~\eqref{eq:n} and ~\eqref{eq:m} we can see no common RHP zeroes. And from equations~\eqref{eq:u} and~\eqref{eq:v} we can devise that it is a semi-proper and stable system as the poles are in the LHP.\\
Youla controller design:\\
G(s) is unstable, all internally stabalizing negative controllers are:\\
\begin{align*}
k(s) = (V-QN)^{-1}(U+QM)
\end{align*}
where Q(s) is stable, $Q(s) \in RH_{\infty}$ and
\begin{equation}
V(s=\infty)-Q(s=\infty)N(s=\infty) \neq 0
\label{eq:y}
\end{equation}
Now,
\begin{align*}
V(s=\infty) &= \lim_{s\to\infty}\: \frac{31-12s-3s^2}{3(s+1)^2}\\
	&= -1\\
N(s=\infty) &= \lim_{s\to\infty}\: \frac{s-1}{(s+1)^3}\\
	&= 0
\end{align*}
Substituting in equation~\eqref{eq:y} we get $-1 \neq 0$. Hence, it is possible to design a stabalizing Youla controller. \\
Let $Q(s) = \frac{1}{s+3}$ then, $k(s) = \frac{U+QM}{V-QN}$\\
$\bm{<Insert Matlab Results here>}$ \\\\

\begin{figure}[htb]
  \centering
  \tikzstyle{block}     = [draw, rectangle, minimum height=1cm, minimum width=1.6cm]
    \tikzstyle{branch}    = [circle, inner sep=0pt, minimum size=1mm, fill=black, draw=black]
    \tikzstyle{connector} = [->, thick]
    \tikzstyle{dummy}     = [inner sep=0pt, minimum size=0pt]
    \tikzstyle{inout}     = []
    \tikzstyle{sum}       = [circle, inner sep=0pt, minimum size=2mm, draw=black, thick]
    \begin{tikzpicture}[auto, node distance=1.6cm, >=stealth']
      \node[block] (G) {$\mathbf{G}$};
      \node[block] (K) [below=of G] {$\mathbf{K}$};
      \node[sum] (s1) [left=of G] {};
      \node[inout] (r) [left=of s1] {$\mathbf{w_1}$};
      \node[sum] (s3) [right= of K] {};
      \node[inout] (n) [right=of s3] {$\mathbf{w_2}$};
      \node[dummy] (d1) [below right=0.1cm and 0.05cm of s1] {$-$};
      \draw[connector] (s1) -- node{$\mathbf{e}_1$}(G);
      \draw[connector] (G) -| node{} (s3);
      \draw[connector] (n) -- (s3);
      \draw[connector] (r) -- (s1);
      \draw[connector] (s3) -- node{$\mathbf{e}_2$} (K);
      \draw[connector] (K) -| (s1);
    \end{tikzpicture}
	  \caption{Closed-loop system with negative feedback}
    \label{fig:blockDiagram1}
\end{figure}
From ~\ref{fig:blockDiagram1} we can derive the following Transfer functions:
\begin{align*}
\bm{TF}_1 &= (\bm{I}+\bm{K}\bm{G})^{-1} \\
\bm{TF}_2 &= -\bm{K}\:(\bm{I}+\bm{G}\bm{K})^{-1} \\
\bm{TF}_3 &= \bm{G}(\bm{I}+\bm{K}\bm{G})^{-1} \\
\bm{TF}_4 &= (\bm{I}+\bm{G}\bm{K})^{-1} 
\end{align*}
$\bm{<Insert Matlab Results (Step Response) here>}$ 
\chapter{Stability and LFT}
\section{Stability and LFT}
\section{Linear fractional transformation}
Using the Block diagram~\ref{fig:blockDiagram} and equation~\eqref{eq:T} we can write:\\
\begin{align*}
\bm{\mathcal{F}}_l(\bm{P},\bm{K}) = \bm{P}_{11} + \bm{P}_{12}\bm{K}(\bm{I}-\bm{P}_{22}\bm{K})^{-1}\: \bm{P}_{21}\\
\end{align*}
where, $\bm{P}_{11}=\bm{D}$, $\bm{P}_{12}=\bm{C}$, $\bm{P}_{21}=\bm{C}$, $\bm{P}_{22}=\bm{A}$ and $\bm{K}=\frac{1}{s}\bm{I}$
\\
\begin{figure}[htb]
  \centering
  \tikzstyle{block}     = [draw, rectangle, minimum height=1cm, minimum width=1.2cm]
    \tikzstyle{branch}    = [circle, inner sep=0pt, minimum size=1mm, fill=black, draw=black]
    \tikzstyle{connector} = [->, thin]
    \tikzstyle{dummy}     = [inner sep=0pt, minimum size=0pt]
    \tikzstyle{inout}     = []
    \tikzstyle{sum}       = [circle, inner sep=0pt, minimum size=2mm, draw=black, thick]
    \begin{tikzpicture}[auto, node distance=1cm, >=stealth']
      \node[block] (P) {$\frac{D}{B}\:\frac{C}{A}$};
      \node[block] (K) [below=of P] {$\frac{1}{s}\bm{I}$};
      \node[inout] (w) [left=of P] {$\bm{u}$};
      \node[inout] (zeta) [right=of P] {$\bm{y}$};
      \draw[->] (K.west) -| ++(-1,1) node {$\bm{\:\:\:\:\:x}$} |- (P.210);
      \draw[->] (P.-30) -| ++(1,-1) node {$\bm{\:\:\:\:\:\dot{x}}$} |- (K.east);
 	 \draw[connector] (P.0) -- (zeta);
	 \draw[connector] (w) -- (P.180);
    \end{tikzpicture}
	  \caption{Lower LFT}
    \label{fig:LFT1}
\end{figure} \\
\begin{figure}[htb]
  \centering
  \tikzstyle{block}     = [draw, rectangle, minimum height=1cm, minimum width=1.2cm]
    \tikzstyle{branch}    = [circle, inner sep=0pt, minimum size=1mm, fill=black, draw=black]
    \tikzstyle{connector} = [->, thin]
    \tikzstyle{dummy}     = [inner sep=0pt, minimum size=0pt]
    \tikzstyle{inout}     = []
    \tikzstyle{sum}       = [circle, inner sep=0pt, minimum size=2mm, draw=black, thick]
    \begin{tikzpicture}[auto, node distance=1cm, >=stealth']
      \node[block] (P) {$\frac{A}{C}\:\frac{B}{D}$};
      \node[block] (K) [above=of P] {$\frac{1}{s}\bm{I}$};
      \node[inout] (w) [left=of P] {$\bm{u}$};
      \node[inout] (zeta) [right=of P] {$\bm{y}$};
      \draw[->] (K.west) -| (-1.5,1) node {$\bm{\:\:\:\:\:x}$} |- (P.150);
      \draw[->] (P.30) -| (1.5,1) node {$\bm{\:\:\:\:\:\dot{x}}$} |- (K.east);
 	 \draw[connector] (P.0) -- (zeta);
	 \draw[connector] (w) -- (P.180);
    \end{tikzpicture}
	  \caption{Upper LFT}
    \label{fig:LFT2}
\end{figure} \\
Considering only the Figure~\ref{fig:LFT2},
\begin{align*}
\bm{G}(s) &= \bm{F}_u(\bm{P},\frac{1}{s}\bm{I}) \\
\end{align*}
where
\begin{align*}
\bm{P} &= 
\begin{bmatrix}
\bm{A} & \bm{B}\\
\bm{C} & \bm{D}\\
\end{bmatrix}
\end{align*}
then,
\begin{align*}
\bm{G}(w) &= \bm{F}_u(\hat{\bm{P}},\frac{1}{w}\bm{I}) \\
\end{align*}
where
\begin{align*}
\hat{\bm{P}} &= 
\begin{bmatrix}
\hat{\bm{A}} & \hat{\bm{B}} \\
\hat{\bm{C}} & \hat{\bm{D}} \\
\end{bmatrix}
\end{align*}
we have,
\begin{align*}
\bm{G}(s) = \bm{F}_u(\bm{P},\bm{F}_u(\bm{N},\frac{1}{w}\bm{I}) = \bm{F}_u(\hat{\bm{P}},\frac{1}{w}\bm{I}) = \bm{G}(w) = \hat{\bm{G}}(s)
\end{align*}
with
\begin{align*}
w &= \frac{as+b}{cs+d}\\
s &= \frac{b-dw}{cw-a}\\
\frac{1}{s} &= \frac{cw-a}{b-dw}\\
\frac{1}{s}\bm{I} &= \bm{F}_u(\bm{N},\frac{1}{w}\bm{I})\\
	&= \bm{N}_{22} + \bm{N}_{21}\frac{1}{w}(\bm{I}-\frac{1}{w}\bm{N}_{11})^{-1}\bm{N}_{12}\\
	&= \bm{N}_{22} + \bm{N}_{21}(w\bm{I}-\bm{N}_{11})^{-1}\bm{N}_{12}\\
	&= (\frac{cw-a}{b-dw}) \bm{I}
\end{align*}
let
\begin{align*}
\frac{cw-a}{b-dw} &= \alpha + \frac{\beta}{b-dw}\\
	&= \frac{\alpha\:b-\alpha\:dw+\beta}{b-dw}
\end{align*}
\begin{align*}
(-\alpha\:d)w + \alpha\:b+\beta = cw-a\\
-\alpha\:d =c \:,\: \alpha\:b+\beta = -a\\
\\
\alpha=\frac{-c}{d} \:,\: \beta = \frac{bc-ad}{d}
\end{align*}
therefore;
\begin{align*}
\frac{1}{s}\bm{I} &=  (\frac{cw-a}{b-dw}) \bm{I}\\
	&= \alpha\bm{I} + \frac{\beta}{b-dw}\bm{I}\\
	&= \frac{-c}{d}\bm{I} +  \frac{bc-ad}{d(b-dw)}\\
	&= \bm{N}_{22} + \bm{N}_{21}\frac{1}{w}(\bm{I}-\frac{1}{w}\bm{N}_{11})^{-1}\bm{N}_{12}
\end{align*}
let,
\begin{equation}
\bm{N}_{22}= \frac{-c}{d}\bm{I}
\label{eq:n22}
\end{equation}
and
\begin{equation}
\bm{N}_{11}= \frac{b}{d}\bm{I}
\label{eq:n11}
\end{equation}
\begin{align*}
\bm{N}_{21}\frac{1}{w}(\bm{I}-\frac{b}{dw}\bm{I})^{-1}\bm{N}_{12} &= \frac{bc-ad}{d(b-dw)}\bm{I} \\
\bm{N}_{21}\frac{1}{w}(\frac{dw}{dw-b})^{-1}\bm{N}_{12} &= \frac{bc-ad}{d(b-dw)}\bm{I} \\
\bm{N}_{21}\bm{N}_{12}(\frac{dw}{dw-b}) &= \frac{-1}{d}(\frac{bc}{d}-a)\\
\end{align*}
let,
\begin{equation}
\bm{N}_{12}= \frac{1}{d}\bm{I}
\label{eq:n12}
\end{equation}
and
\begin{equation}
\bm{N}_{21}= -(\frac{bc}{d}-a)\bm{I}
\label{eq:n21}
\end{equation}
thus, in $\frac{1}{s}\bm{I} = \bm{F}_u(\bm{N},\frac{1}{w}\bm{I})$\\
where\\
\begin{align*}
\bm{N}=
\begin{bmatrix}
\frac{b}{d}\bm{I} &  \frac{1}{d}\bm{I}\\
-(\frac{bc}{d}-a)\bm{I} & \frac{-c}{d}\bm{I}
\end{bmatrix}
\end{align*}
Now,
\begin{align*}
\bm{G}(s)&=\bm{F}_u(
\begin{bmatrix}
\bm{A} & \bm{B}\\
\bm{C} & \bm{D}
\end{bmatrix}, \frac{1}{s}\bm{I})\\
&=\bm{F}_u(
\begin{bmatrix}
\bm{A} & \bm{B}\\
\bm{C} & \bm{D}
\end{bmatrix}, \bm{F}_u(\bm{N},\frac{1}{w}\bm{I}))\\
&= \bm{C} \:\bm{F}_u(\bm{N},\frac{1}{w}\bm{I}) [\bm{I} - \bm{A}\bm{F}_u(\bm{N},\frac{1}{w}\bm{I})]^{-1} \: \bm{B} + \bm{D}\\
\bm{G}(w) &= \hat{\bm{C}}\frac{1}{w}\bm{I} (w\bm{I} - \hat{\bm{A}})^{-1} \hat{\bm{B}} + \hat{\bm{D}}\\
&=\bm{F}_u(
\begin{bmatrix}
\hat{\bm{A}} & \hat{\bm{B}}\\
\hat{\bm{C}} & \hat{\bm{D}}
\end{bmatrix}, \frac{1}{w}\bm{I})\\
\end{align*}
For Lower LFT according to block diagram~\ref{fig:LFT1}:
\begin{align*}
\bm{G}(s)&=\bm{F}_l(
\begin{bmatrix}
\bm{D} & \bm{C}\\
\bm{B} & \bm{A}
\end{bmatrix}, \frac{1}{s}\bm{I})\\
&= \bm{F}_l(
\begin{bmatrix}
\bm{D} & \bm{C}\\
\bm{B} & \bm{A}
\end{bmatrix}, \bm{F}_l\bm{N},\frac{1}{w}\bm{I}))\\
&=\bm{F}_l(
\begin{bmatrix}
\hat{\bm{D}} & \hat{\bm{C}}\\
\hat{\bm{B}} & \hat{\bm{A}}
\end{bmatrix}, \frac{1}{w}\bm{I})\\
\end{align*}
where,
\begin{align*}
\bm{N}=
\begin{bmatrix}
 \frac{-c}{d}\bm{I} & (\frac{ad-bc}{d})\bm{I}\\
\frac{1}{d}\bm{I} & \frac{b}{d}\bm{I}
\end{bmatrix}
\end{align*}
\begin{align*}
\hat{\bm{D}} &= \bm{D}-\bm{C}(\frac{c}{d})(\bm{I}+\bm{A}\frac{c}{d})^{-1}\bm{B}\\
	&= \bm{D}-\frac{c}{d}\bm{C}(d\bm{I}+c\bm{A})^{-1}.d\bm{B}\\
	&= \bm{D}-c\bm{C}(d\bm{I}+c\bm{A})^{-1}\bm{B}\\
\hat{\bm{C}} &= \bm{C}(\bm{I}+\frac{c}{d}\bm{A})^{-1}(\frac{ad-bc}{d})\bm{I}\\
	&= \bm{C}(d\bm{I}+c\bm{A})^{-1}d(\frac{ad-bc}{d})\bm{I}\\
	&= (ad-bc)\bm{C}(d\bm{I}+c\bm{A})^{-1}\\
\hat{\bm{B}} &= \frac{1}{d}(\bm{I}+\bm{A}\frac{c}{d})\bm{B}\\
	&= (d\bm{I}+c\bm{A})^{-1}\bm{B}\\
\hat{\bm{A}} &= \frac{b}{d}\bm{I}+(\frac{1}{d})\bm{A}(\bm{I}+\frac{c}{d}\bm{A})^{-1}(\frac{ad-bc}{d})\\
	&=\frac{db\bm{I}+\bm{A}(\bm{I}+\frac{c}{d}\bm{A})^{-1}(ad-bc)}{d^2}\\
	&=\frac{db\bm{I}+\bm{A}(d\bm{I}+c\bm{A})^{-1}(ad-bc)}{d}\\
	&= b\bm{I}+\bm{A}(d\bm{I}+c\bm{A})^{-1}(a-\frac{bc}{d})\\
	&= a\bm{A}(d\bm{I}+c\bm{A})^{-1}-\frac{bc}{d}(d\bm{I}+c\bm{A})^{-1} + b\bm{I}\\
	&= a\bm{A}(d\bm{I}+c\bm{A})^{-1}+b[\bm{I}-\frac{c}{d}\bm{A}(d\bm{I}+c\bm{A})^{-1}]\\
	&= (a\bm{A}+b\bm{I})(d\bm{I}+c\bm{A})^{-1}
\end{align*}
b.i) Controllability:
\begin{align*}
& \hat{\bm{u}}_{pi} \neq 0 , \forall i \in [1, n]\\
& \hat{u}_{pi}=\hat{\bm{q}}_{i}^H\:\hat{\bm{B}}\\
& where,\:\: \hat{\bm{q}}_{i}^H \: is\: the\: i^{th}\: Eigenvector \:of \hat{\bm{A}}
\end{align*}
Now,
\begin{align*}
&\hat{\bm{u}}_{pi} = \hat{\bm{q}}_{i}^H(d\bm{I}+c\bm{A})^{-1}\bm{B}\\
& \hat{\bm{q}}_{i}^H = \bm{q}_{i}^H\\
& \hat{\bm{u}}_{pi} = \bm{q}_{i}^H\hat{\bm{B}}\\
& \hat{\bm{u}}_{pi} = \bm{q}_{i}^H(d\bm{I}+c\bm{A})^{-1}\bm{B} \:\:\: and \:\:\: \bm{u}_{pi} = \bm{q}_{i}^H\bm{B}\\
\end{align*}
b.ii) Observability:\\\\
$(\hat{\bm{A}},\hat{\bm{C}})$ is observable iff, $\hat{\bm{y}}_{pi}=\hat{\bm{C}}\hat{\bm{t}}_{i} \neq 0$, $\forall$  i$\in$[i,n]\\
\\
Similarly we can prove that the same right Eigenvectors diagonalize $\bm{A}$ and $(a\bm{A}+b\bm{I})(d\bm{I}+c\bm{A})^{-1}$\\
\\ 
thus, $\hat{\bm{t}}_{i}=\bm{t}_{i}$\\ 
and, $\hat{\bm{y}}_{pi}=(ad-bc)\bm{C}(d\bm{I}+c\bm{A})^{-1}\bm{t}_{i} \neq 0$\\
Hence, $ad-bc\neq 0$ and $(d\bm{I}+c\bm{A})^{-1} \neq 0$ for a finite $\bm{A}$
\section{References}
by inserting equations~\eqref{eq:n22},~\eqref{eq:n11},~\eqref{eq:n12},~\eqref{eq:n21} 
Please use the bibtex library file called literature.bib in main folder of this template. A simple tool to manage your references is JabRef. Note that there are differences between Books~\cite{Sko05}, Journal articles~\cite{Rue14} and contributions to Conferences~\cite{Mis13}.

%%%%%%%%%%%%%%%%%%%%%%%%%%%%% Content ends here %%%%%%%%%%%%%%%%%%%%%%%%%%%%%

\bibliographystyle{abbrv}
\bibliography{literature}

\end{document}